more

theories/Subst.v
@@ -1,6 +1,8 @@
+From Hammer Require Import Tactics.
 From Coq Require Import String.
 From LambdaST Require Import
   Terms
+  FV
   Types.
 
 Definition subst_str (x y z : string) := if eqb z x then y else z.
@@ -14,15 +16,15 @@ Fixpoint subst_var (e : term) (x : string) (y : string) : term :=
   | TmUnit =>
       e
   | TmVar z =>
-      TmVar (subst_str x y z)
+      TmVar (if eqb z y then x else z)
   | TmComma lhs rhs =>
       TmComma (subst_var lhs x y) (subst_var rhs x y)
   | TmSemic lhs rhs =>
       TmSemic (subst_var lhs x y) (subst_var rhs x y)
-  | TmLet bind bound body =>
-      let subst_bound := subst_var bound x y in
-      let subst_body := if eqb bind x then (* shadowing *) body else (* no shadowing *) subst_var body x y in
-      TmLet bind subst_bound subst_body
+  | TmLet x' e e' => TmLet x' (subst_var e x y) (subst_var e' x y)
+      (* let subst_bound := subst_var bound x y in *)
+      (* let subst_body := if eqb bind x then shadowing body else no shadowing subst_var body x y in *)
+      (* TmLet bind subst_bound subst_body *)
   | TmLetPar lhs rhs bound body =>
       let subst_bound := subst_str x y bound in
       let subst_body := if (eqb x lhs || eqb x rhs)%bool then body else subst_var body x y in
@@ -31,5 +33,15 @@ Fixpoint subst_var (e : term) (x : string) (y : string) : term :=
       let subst_bound := subst_str x y bound in
       let subst_body := if (eqb x lhs || eqb x rhs)%bool then body else subst_var body x y in
       TmLetCat t lhs rhs subst_bound body
+  | TmInl e => TmInl (subst_var e x y)
+  | TmInr e => TmInr (subst_var e x y)
+  | TmPlusCase eta r z x' e1 y' e2 => TmPlusCase eta r z x' (subst_var e1 x y) y' (subst_var e2 x y)
   end.
 Arguments subst_var e/ x y.
+
+
+(* TODO: will. *)
+Theorem subst_not_fv : forall e x y,
+    ~(fv e y) -> e = subst_var e x y.
+Proof.
+Admitted.
